renaming

theories/CodegenWasm/LambdaANF_to_Wasm.v
@@ -420,12 +420,12 @@ Fixpoint create_case_nested_if_chain (boxed : bool) (v : immediate) (es : list (
 
 (* ***** TRANSLATE EXPRESSIONS (except fundefs) ****** *)
 
-Fixpoint translate_exp (nenv : name_env) (cenv : ctor_env) (lenv: localvar_env) (fenv : fname_env) (e : exp) : error (list basic_instruction) :=
+Fixpoint translate_body (nenv : name_env) (cenv : ctor_env) (lenv: localvar_env) (fenv : fname_env) (e : exp) : error (list basic_instruction) :=
    match e with
    | Efun fundefs e' => Err "unexpected nested function definition"
    | Econstr x tg ys e' =>
-      following_instr <- translate_exp nenv cenv lenv fenv e' ;;
-      x_var <- translate_var nenv lenv x "translate_exp constr";;
+      following_instr <- translate_body nenv cenv lenv fenv e' ;;
+      x_var <- translate_var nenv lenv x "translate_body constr";;
       match ys with
       | [] => Ret ([ BI_const (nat_to_value (Pos.to_nat tg)) (* Nullary constructor *)
                   (* Unboxed representation ( (tag << 1) + 1 ) *)
@@ -456,7 +456,7 @@ Fixpoint translate_exp (nenv : name_env) (cenv : ctor_env) (lenv: localvar_env) 
         match arms with
         | [] => Ret ([], [])
         | (t, e)::tl =>
-            instrs <- translate_exp nenv cenv lenv fenv e ;;
+            instrs <- translate_body nenv cenv lenv fenv e ;;
             '(arms_boxed, arms_unboxed) <- translate_case_branch_expressions tl ;;
             arity <- get_ctor_arity cenv t ;;
             if arity =? 0 then
@@ -465,7 +465,7 @@ Fixpoint translate_exp (nenv : name_env) (cenv : ctor_env) (lenv: localvar_env) 
               Ret ((t, instrs) :: arms_boxed, arms_unboxed)
         end
       in
-      x_var <- translate_var nenv lenv x "translate_exp case" ;;
+      x_var <- translate_var nenv lenv x "translate_body case" ;;
       '(arms_boxed, arms_unboxed) <- translate_case_branch_expressions arms ;;
       Ret ([ BI_get_local x_var
            ; BI_const (nat_to_value 1)
@@ -477,9 +477,9 @@ Fixpoint translate_exp (nenv : name_env) (cenv : ctor_env) (lenv: localvar_env) 
            ])
 
    | Eproj x tg n y e' =>
-      following_instr <- translate_exp nenv cenv lenv fenv e' ;;
-      y_var <- translate_var nenv lenv y "translate_exp proj y";;
-      x_var <- translate_var nenv lenv x "translate_exp proj x";;
+      following_instr <- translate_body nenv cenv lenv fenv e' ;;
+      y_var <- translate_var nenv lenv y "translate_body proj y";;
+      x_var <- translate_var nenv lenv x "translate_body proj x";;
 
       Ret ([ BI_get_local y_var
            ; BI_const (nat_to_value (((N.to_nat n) + 1) * 4)) (* skip ctor_id and previous constr arguments *)
@@ -489,8 +489,8 @@ Fixpoint translate_exp (nenv : name_env) (cenv : ctor_env) (lenv: localvar_env) 
            ] ++ following_instr)
 
    | Eletapp x f ft ys e' =>
-      x_var <- translate_var nenv lenv x "translate_exp proj x";;
-      following_instr <- translate_exp nenv cenv lenv fenv e' ;;
+      x_var <- translate_var nenv lenv x "translate_body proj x";;
+      following_instr <- translate_body nenv cenv lenv fenv e' ;;
       instr_call <- translate_call nenv lenv fenv f ys false;;
 
       Ret (instr_call ++ [ BI_get_global result_out_of_mem
@@ -504,8 +504,8 @@ Fixpoint translate_exp (nenv : name_env) (cenv : ctor_env) (lenv: localvar_env) 
    | Eapp f ft ys => translate_call nenv lenv fenv f ys true
 
    | Eprim_val x p e' =>
-       following_instrs <- translate_exp nenv cenv lenv fenv e' ;;
-       x_var <- translate_var nenv lenv x "translate_exp prim val" ;;
+       following_instrs <- translate_body nenv cenv lenv fenv e' ;;
+       x_var <- translate_var nenv lenv x "translate_body prim val" ;;
        val <- translate_primitive p ;;
        Ret ([ BI_const (N_to_value page_size)
             ; BI_call grow_mem_function_idx
@@ -529,7 +529,7 @@ Fixpoint translate_exp (nenv : name_env) (cenv : ctor_env) (lenv: localvar_env) 
    | Eprim x p ys e' => Err "translating prim to Wasm not supported yet"
 
    | Ehalt x =>
-     x_var <- translate_var nenv lenv x "translate_exp halt";;
+     x_var <- translate_var nenv lenv x "translate_body halt";;
      Ret [ BI_get_local x_var; BI_set_global result_var; BI_return ]
    end.
 
@@ -575,7 +575,7 @@ Definition translate_function (nenv : name_env) (cenv : ctor_env) (fenv : fname_
   let lenv := create_local_variable_mapping (args ++ locals) in
 
   fn_idx <- translate_var nenv fenv f "translate function" ;;
-  body_res <- translate_exp nenv cenv lenv fenv body ;;
+  body_res <- translate_body nenv cenv lenv fenv body ;;
   Ret {| fidx := fn_idx
        ; export_name := function_export_name nenv f
        ; type := Tf (map (fun _ => T_i32) args) []
@@ -654,7 +654,7 @@ Definition LambdaANF_to_Wasm (nenv : name_env) (cenv : ctor_env) (e : exp) : err
                end;;
   let main_vars := collect_local_variables main_expr in
   let main_lenv := create_local_variable_mapping main_vars in
-  main_instr <- translate_exp nenv cenv main_lenv fname_mapping main_expr ;;
+  main_instr <- translate_body nenv cenv main_lenv fname_mapping main_expr ;;
 
   let main_function := {| fidx := main_function_idx
                         ; export_name := main_function_name
